veric/initialize.v
@@ -16,7 +16,6 @@ Require Import veric.Clight_lemmas.
 Require Import veric.initial_world.
 
 
-
 Lemma alloc_globals_app:
    forall F V (ge: Genv.t F V) m m2 vs vs',
   Genv.alloc_globals ge m (vs++vs') = Some m2 <->
@@ -94,6 +93,87 @@ Proof.
     simpl. auto.
 Qed.
 
+
+(* Inductive init_data: Type :=
+  | Init_int8: int -> init_data
+  | Init_int16: int -> init_data
+  | Init_int32: int -> init_data
+  | Init_float32: float -> init_data
+  | Init_float64: float -> init_data
+  | Init_space: Z -> init_data
+  | Init_addrof: ident -> int -> init_data.  (**r address of symbol + offset *)
+Definition store_init_data (m: mem) (b: block) (p: Z) (id: init_data) : option mem :=
+  match id with
+  | Init_int8 n => Mem.store Mint8unsigned m b p (Vint n)
+  | Init_int16 n => Mem.store Mint16unsigned m b p (Vint n)
+  | Init_int32 n => Mem.store Mint32 m b p (Vint n)
+  | Init_float32 n => Mem.store Mfloat32 m b p (Vfloat n)
+  | Init_float64 n => Mem.store Mfloat64 m b p (Vfloat n)
+  | Init_addrof symb ofs =>
+      match find_symbol ge symb with
+      | None => None
+      | Some b' => Mem.store Mint32 m b p (Vptr b' ofs)
+      end
+  | Init_space n => Some m
+  end.
+*)
+
+Definition mapsto_zeros (n: Z) : spec :=
+     fun (rsh sh: Share.t) (l: address) =>
+          allp (jam (adr_range_dec l (Zmax n 0))
+                                  (fun l' => yesat NoneP (VAL (Byte Byte.zero)) rsh sh l')
+                                  noat).
+
+Definition init_data2pred (ge: Genv.t fundef type) (d: init_data) : spec :=
+ match d with
+  | Init_int8 i => address_mapsto Mint8unsigned (Vint (Int.zero_ext 8 i))
+  | Init_int16 i => address_mapsto Mint16unsigned (Vint (Int.zero_ext 16 i))
+  | Init_int32 i => address_mapsto Mint32 (Vint i) 
+  | Init_float32 r =>  address_mapsto Mfloat32 (Vfloat ((Float.singleoffloat r)))
+  | Init_float64 r =>  address_mapsto Mfloat64 (Vfloat r)
+  | Init_space n => mapsto_zeros n 
+  | Init_addrof symb ofs =>
+       match Genv.find_symbol ge symb with
+       | None => mapsto_zeros (Genv.init_data_size d)
+       | Some b' => address_mapsto Mint32 (Vptr b' ofs)
+       end
+ end.
+
+Fixpoint init_data_list2pred  (ge: Genv.t fundef type)  (dl: list init_data) (sh: share) (b: block) (ofs: Z) : pred rmap :=
+  match dl with
+  | d::dl' => 
+      sepcon (init_data2pred ge d extern_retainer sh (b, ofs)) 
+                  (init_data_list2pred ge dl' sh b (ofs + Genv.init_data_size d))
+  | nil => emp
+ end.
+
+Definition readonly2share (rdonly: bool) : share :=
+  if rdonly then Share.Lsh else Share.top.
+
+Definition globvar2pred (ge: Genv.t fundef type) (idv: ident * globvar type) : pred rmap :=
+  match Genv.find_symbol ge (fst idv) with
+  | None => emp
+  | Some b => if (gvar_volatile (snd idv))
+                       then  TT
+                       else    init_data_list2pred ge (gvar_init (snd idv))
+                                   (readonly2share (gvar_readonly (snd idv))) b 0
+ end.
+
+Definition globvars2pred (ge: Genv.t fundef type) (vl: list (ident * globvar type)) : pred rmap :=
+  fold_right sepcon emp (map (globvar2pred ge) vl).
+
+Lemma globvars2pred_rev:
+  forall ge l, globvars2pred ge (rev l) = globvars2pred ge l.
+Proof.
+ intros. unfold globvars2pred. 
+ rewrite map_rev.
+  rewrite fold_left_rev_right.
+ rewrite fold_symmetric.
+ f_equal. extensionality x y; apply sepcon_comm.
+ intros; apply sepcon_assoc.
+ intros; apply sepcon_comm.
+Qed.
+
 Lemma writable_blocks_rev:
   forall rho l, writable_blocks l rho = writable_blocks (rev l) rho.
 Proof.
@@ -113,134 +193,6 @@ Lemma add_variables_nextblock:
 Proof.
 Admitted.
 
-
-Lemma global_initializers:
-  forall prog G m n,
-     list_norepet (prog_defs_names prog) ->
-    match_fdecs (prog_funct prog) G ->
-    Genv.init_mem prog = Some m ->
-     app_pred 
-      (writable_blocks (map (initblocksize type) (prog_vars prog))
-          (base.empty_environ (Genv.globalenv prog)))
-  (inflate_initial_mem m (initial_core (Genv.globalenv prog) G n)).
-Proof.
- intros until n. intros ? SAME_IDS ?.
- assert (IOK: initial_rmap_ok m (initial_core (Genv.globalenv prog) G n))
-      by (apply initial_core_ok; auto).
-  unfold Genv.init_mem in H0.
-  unfold Genv.globalenv in *.
-  destruct prog as [fl main vl].
-  simpl in *.
-  remember (Genv.add_globals (Genv.empty_genv fundef type) fl) as gev.
-  rewrite <- (rev_involutive fl) in *.
-  rewrite alloc_globals_rev_eq in H0.
-  forget (rev fl) as vl'. clear fl; rename vl' into vl.
-  unfold prog_vars. simpl.
-  rewrite <- rev_prog_vars'.
-  rewrite map_rev. rewrite <- writable_blocks_rev.
-  assert (exists ul, gev = Genv.add_globals (Genv.empty_genv fundef type) (rev vl ++ ul) /\ 
-                                            list_norepet (map (@fst _ _) (rev vl ++ ul))).
-  exists nil; rewrite <- app_nil_end; auto.
-  clear Heqgev H.
-  revert m H0 H1 IOK SAME_IDS; induction vl; simpl; intros.
- apply resource_at_empty2.
- intro l.
- unfold inflate_initial_mem.
- rewrite resource_at_make_rmap.
- unfold inflate_initial_mem'.
-  inv H0.
- unfold access_at, empty. simpl. rewrite ZMap.gi. apply NO_identity.
-(*
- invSome.
- destruct a; destruct g.
- apply (H3 m0).
- case_eq (initblocksize type a); intros.
- specialize (IHvl _ H0).
- unfold writable_block.
- normalize.
- unfold initblocksize in H.
- destruct a. inv H.
- unfold Genv.alloc_variable in H3.
- simpl in H3.
- revert H3; case_eq (alloc m0 0 (Genv.init_data_list_size (gvar_init g))); intros.
- invSome. invSome.
- unfold empty_environ at 1. simpl ge_of. unfold filter_genv.
- destruct H1 as [ul [? ?]].
- spec IHvl.
-  exists ((i,g)::ul).
- rewrite app_ass in H1,H2; split; auto.
- assert (Genv.find_symbol gev i = Some b).
- clear - H0 H H1 H2 H9.
- apply alloc_result in H. subst.
- rewrite <- alloc_variables_rev_eq in H0. 
- apply Genv.alloc_variables_nextblock in H0.
- rewrite H0. clear - H2 H9.
- rewrite app_ass in *. simpl app in *.
- simpl nextblock. rewrite <- H9.
- apply add_variables_nextblock; auto. 
- rewrite H4.
- exists (Vptr b Int.zero, match type_of_global gev b with
-      | Some t => t
-      | None => Tvoid
-      end).
- normalize.
- exists (b, 0).
- normalize; exists Share.bot.
- normalize.
- split.
- simpl. split.
- destruct (type_of_global gev b); auto.
- f_equal; rewrite Int.signed_zero; auto.
- rewrite sepcon_comm.
- assert (b>0). apply alloc_result in H. subst; apply nextblock_pos.
- apply (mem_alloc_juicy _ _ _ _ _ H
-                    (initial_core gev G n)
-                   (writable_blocks (map (initblocksize type) vl) (empty_environ gev))
-                  IOK IOK) in IHvl.
- rewrite Zminus_0_r in IHvl.
- apply (store_zeros_lem _ _ _ _ H3 H7 _ IOK IOK) in IHvl.
- apply (store_init_data_list_lem _ _ _ _ _ _ _ _ H5 H7 _ IOK IOK) in IHvl.
- rewrite <- (Zminus_0_r  (Genv.init_data_list_size (gvar_init g))) in IHvl.
- assert (Genv.perm_globvar g = Writable) by admit. (* need to generalize this! *)
- rewrite H8 in *.
- apply (drop_perm_writable_lem _ _ _ _ _ H6 H7 _ IOK IOK) in IHvl.
- rewrite Zminus_0_r in IHvl.
- apply IHvl.
-Qed. *)
-Admitted.
-
-
-Definition bump_nextvar {F V} (ge: Genv.t F V)  : Genv.t F V.
-intros.
-apply (@Genv.mkgenv F V
-    ge.(Genv.genv_symb)
-    ge.(Genv.genv_funs)
-    ge.(Genv.genv_vars)
-    (ge.(Genv.genv_next) + 1)); intros; destruct ge; simpl in *; auto.
-unfold block in *. omega.
-destruct (genv_symb_range _ _ H); split; unfold block in*; omega.
-pose proof (genv_funs_range _ _ H); omega.
-pose proof (genv_vars_range _ _ H); omega.
-eapply genv_funs_vars; eauto.
-apply genv_vars_inj with b; auto.
-Defined.
-
-Lemma disj_no_fun:
-  forall (fs: list (AST.ident * globdef fundef type)) ids, 
-       list_disjoint (map (@fst _ _) fs) ids ->
-       forall i, In i ids ->
-      (Genv.genv_symb (Genv.add_globals (Genv.empty_genv _ _) fs)) ! i = None.
-Proof.
-intros. spec H i i.
-assert (~In i (map (@fst _ _) fs)). intro. contradiction H; auto.
-clear - H1; rename H1 into H0. unfold Genv.add_globals.
-rewrite fold_right_rev_left. rewrite <- (rev_involutive fs). rewrite In_rev in H0.
-rewrite <- map_rev in H0. remember (rev fs) as fs'; rewrite rev_involutive. clear - H0.
-revert H0; induction fs'; simpl; intros.
-rewrite Maps.PTree.gempty; auto. destruct a; simpl in *.
-rewrite Maps.PTree.gso; [ | intro; subst; intuition]. 
-apply IHfs'. contradict H0; auto.
-Qed.
 
 Definition upto_block' (b: block) (w: rmap) :=
   fun loc => if zlt (fst loc) b then w @ loc else NO Share.bot.
@@ -285,3 +237,673 @@ Proof.
  if_tac. repeat rewrite core_resource_at. rewrite <- level_core; apply resource_at_approx.
 apply resource_at_approx.
 Defined.
+
+
+Lemma split_range: 
+  forall phi base n, 
+    (forall loc, adr_range base n loc -> 
+       match phi @ loc with YES _ _ k _ => isVAL k | _ => True end) ->
+   exists phi1, exists phi2, 
+      join phi1 phi2 phi /\
+      forall loc, if adr_range_dec base n loc then identity (phi2 @ loc) 
+                                                      else identity (phi1 @ loc).
+Admitted.
+
+
+Definition load_store_init_data1 (ge: Genv.t fundef type) (m: mem) (b: block) (p: Z) (d: init_data) : Prop :=
+  match d with
+  | Init_int8 n =>
+      Mem.load Mint8unsigned m b p = Some(Vint(Int.zero_ext 8 n))
+  | Init_int16 n =>
+      Mem.load Mint16unsigned m b p = Some(Vint(Int.zero_ext 16 n))
+  | Init_int32 n =>
+      Mem.load Mint32 m b p = Some(Vint n)
+  | Init_float32 n =>
+      Mem.load Mfloat32 m b p = Some(Vfloat(Float.singleoffloat n))
+  | Init_float64 n =>
+      Mem.load Mfloat64 m b p = Some(Vfloat n)
+  | Init_addrof symb ofs =>
+      Mem.load Mint32 m b p = Some 
+             match Genv.find_symbol ge symb with  
+                | Some b' => Vptr b' ofs 
+                | None => Vint Int.zero
+              end        
+  | Init_space n =>
+      forall z, 0 <= z < Zmax n 0 -> 
+           Mem.load Mint8unsigned m b (p+z) = Some (Vint Int.zero)
+  end.
+
+Definition initializer_aligned (z: Z) (d: init_data) : bool :=
+  match d with
+  | Init_int16 n => Zeq_bool (z mod 2) 0
+  | Init_int32 n => Zeq_bool (z mod 4) 0
+  | Init_float32 n =>  Zeq_bool (z mod 4) 0
+  | Init_float64 n =>  Zeq_bool (z mod 8) 0
+  | Init_addrof symb ofs =>  Zeq_bool (z mod 4) 0
+  | _ => true
+  end.
+  
+Fixpoint initializers_aligned (z: Z) (dl: list init_data) : bool :=
+  match dl with 
+  | nil => true 
+  | d::dl' => andb (initializer_aligned z d) (initializers_aligned (z + Genv.init_data_size d) dl')
+  end.
+
+Lemma load_store_init_data_lem1:
+  forall {ge m1 b D m2 m3},
+   Genv.store_zeros m1 b 0 (Genv.init_data_list_size D) = Some m2 ->
+   Genv.store_init_data_list ge m2 b 0 D = Some m3 ->
+   forall dl' a dl, dl' ++ a :: dl = D ->
+   load_store_init_data1 ge m3 b (Genv.init_data_list_size dl') a.
+Proof.
+  intros.
+  pose proof (Genv.store_init_data_list_charact _ _ _ _ _ H0).
+  subst D.
+  change (Genv.init_data_list_size dl') with (0 + Genv.init_data_list_size dl'). 
+  forget 0 as z.
+  assert (forall z', z <= z' < z + Genv.init_data_list_size (dl' ++ a :: dl) ->
+               Mem.load Mint8unsigned m2 b z' = Some (Vint Int.zero)).
+  clear - H. admit.
+  clear H m1.
+  revert z m2 H0 H1 H2; induction dl'; intros.
+  simpl app in *. simpl Genv.init_data_list_size in *.
+  replace (z+0) with z by omega.
+  destruct a; simpl in H2|-*; try solve [destruct H2; auto]; intros.
+  simpl in H0.
+  rewrite (Genv.store_init_data_list_outside ge dl m2  H0) by (right; simpl; omega).
+  apply H1.
+  simpl.
+  assert (Genv.init_data_list_size dl >= 0) by admit.
+  omega.
+  destruct H2 as [[b' [? ?]] ?].
+  rewrite H. auto. 
+  simpl.
+  simpl in H0. invSome.
+  rewrite Zplus_assoc. apply IHdl' with m; auto.
+  intros.
+  rewrite <- (H1 z').
+  destruct (store_init_data_list_outside' _ _ ge b (a0::nil) m2 z m).
+  simpl. rewrite H0; auto.
+  destruct (H3 b z').
+  destruct H6. simpl in H7. omegaContradiction.
+  destruct H5. clear - H6 H5; unfold access_at,contents_at in *.
+  Transparent load. unfold load. Opaque load.
+  simpl in *. rewrite H6.
+  destruct (valid_access_dec m Mint8unsigned b z' Readable);
+   destruct (valid_access_dec m2 Mint8unsigned b z' Readable);
+  unfold valid_access in *; try congruence.
+  contradiction n. clear - v H5.
+  unfold range_perm, perm in *.
+  destruct v; split; auto; intros.
+  apply (equal_f ) with (b,ofs) in H5. simpl in H5. rewrite H5; auto.
+  contradiction n. clear - v H5.
+  unfold range_perm, perm in *.
+  destruct v; split; auto; intros.
+  apply (equal_f ) with (b,ofs) in H5. simpl in H5. rewrite <- H5; auto.
+  simpl. 
+    assert (Genv.init_data_size  a0 >= 0) by admit.
+  omega.
+  clear - H2.
+  simpl app in H2.
+  forget (dl'++a::dl) as D.
+  simpl in H2. destruct a0; simpl in *; try solve [destruct H2; auto]; intros.
+  auto.
+Qed.
+
+Lemma read_sh_readonly:
+  forall NU, read_sh = mk_lifted (readonly2share true) NU.
+Proof.
+  simpl. unfold read_sh. simpl. f_equal; auto.
+Qed.  
+
+Lemma init_data_lem:
+forall (ge : Genv.t fundef type) (v : globvar type) (b : block) (m1 : mem')
+  (m3 m4 : Memory.mem) (phi0 : rmap) (a : init_data) (z : Z)
+  (w1 wf : rmap),
+   load_store_init_data1 ge m3 b z a ->
+   contents_at m4 = contents_at m3 ->
+   join w1 wf (beyond_block b (inflate_initial_mem m4 phi0)) ->
+   (forall loc : address,
+     if adr_range_dec (b, z) (Genv.init_data_size a) loc
+     then identity (wf @ loc) /\ access_at m4 loc = Some (Genv.perm_globvar v)
+     else identity (w1 @ loc)) ->
+     gvar_volatile v = false ->
+   initializer_aligned z a = true ->
+  (init_data2pred ge a extern_retainer (readonly2share (gvar_readonly v)) (b, z)) w1.
+Proof.
+  intros. rename H4 into AL; rename H3 into VOL.
+  assert (NU: nonunit (readonly2share (gvar_readonly v))).
+  destruct (gvar_readonly v); simpl.
+  admit. (* easy *)
+    admit. (* easy *)
+  Transparent load. 
+  destruct a; unfold init_data2pred; simpl in H; unfold load in H;
+  try (if_tac in H; [ | discriminate H]);
+  try match type of H with Some (decode_val ?ch ?B) = Some (?V) =>
+            exists B; replace V with (decode_val ch B) by (inversion H; auto)
+       end.
+(* Int8 *)
+  repeat split; auto; clear H.
+  apply Zone_divide.
+  intro loc; specialize (H2 loc).
+  simpl in H2. hnf. simpl size_chunk. if_tac; auto.
+  exists NU.
+  destruct H2.
+  apply join_comm in H1.
+  apply (resource_at_join _ _ _ loc) in H1.
+  apply H2 in H1. hnf. rewrite H1.
+  unfold beyond_block. rewrite resource_at_make_rmap.
+  unfold beyond_block'. 
+  rewrite if_false by (  destruct loc; destruct H; subst; simpl; unfold block; omega).
+  unfold inflate_initial_mem. rewrite resource_at_make_rmap.
+  unfold inflate_initial_mem'. rewrite H4.
+ unfold Genv.perm_globvar. rewrite VOL. rewrite preds_fmap_NoneP.
+  destruct (gvar_readonly v);  repeat f_equal; auto.
+  apply read_sh_readonly.
+  rewrite H0.
+  destruct loc; destruct H; subst b0.
+  apply nth_getN; simpl; omega.
+  rewrite H0.
+  destruct loc; destruct H; subst b0.
+  apply nth_getN; simpl; omega.
+  
+  repeat split; auto; clear H.
+  simpl in AL. apply Zmod_divide.  intro Hx; inv Hx. apply Zeq_bool_eq; auto.
+  intro loc; specialize (H2 loc).
+  simpl in H2. simpl size_chunk. hnf; if_tac; auto.
+  exists NU.
+  destruct H2.
+  apply join_comm in H1.
+  apply (resource_at_join _ _ _ loc) in H1.
+  apply H2 in H1. hnf; rewrite H1.
+  unfold beyond_block. rewrite resource_at_make_rmap.
+  unfold beyond_block'.
+  rewrite if_false by (  destruct loc; destruct H; subst; simpl; unfold block; omega).
+  unfold inflate_initial_mem. rewrite resource_at_make_rmap.
+  unfold inflate_initial_mem'. rewrite H4.
+ unfold Genv.perm_globvar. rewrite VOL. rewrite preds_fmap_NoneP.
+  destruct (gvar_readonly v);  repeat f_equal; auto.
+  apply read_sh_readonly.
+  rewrite H0.
+  destruct loc; destruct H; subst b0.
+  apply nth_getN; simpl; omega.
+  rewrite H0.
+  destruct loc; destruct H; subst b0.
+  apply nth_getN; simpl; omega.  
+  repeat split; auto; clear H.
+  simpl in AL. apply Zmod_divide.  intro Hx; inv Hx. apply Zeq_bool_eq; auto.
+  intro loc; specialize (H2 loc).
+  simpl in H2. simpl size_chunk. hnf; if_tac; auto.
+  exists NU.
+  destruct H2.
+  apply join_comm in H1.
+  apply (resource_at_join _ _ _ loc) in H1.
+  apply H2 in H1. hnf; rewrite H1.
+  unfold beyond_block. rewrite resource_at_make_rmap.
+  unfold beyond_block'.
+  rewrite if_false by (  destruct loc; destruct H; subst; simpl; unfold block; omega).
+  unfold inflate_initial_mem. rewrite resource_at_make_rmap.
+  unfold inflate_initial_mem'. rewrite H4.
+ unfold Genv.perm_globvar. rewrite VOL. rewrite preds_fmap_NoneP.
+  destruct (gvar_readonly v);  repeat f_equal; auto.
+  apply read_sh_readonly.
+  rewrite H0.
+  destruct loc; destruct H; subst b0.
+  apply nth_getN; simpl; omega.
+  rewrite H0.
+  destruct loc; destruct H; subst b0.
+  apply nth_getN; simpl; omega.
+
+  repeat split; auto; clear H.
+  simpl in AL. apply Zmod_divide.  intro Hx; inv Hx. apply Zeq_bool_eq; auto.
+  intro loc; specialize (H2 loc).
+  simpl in H2. simpl size_chunk. hnf; if_tac; auto.
+  exists NU.
+  destruct H2.
+  apply join_comm in H1.
+  apply (resource_at_join _ _ _ loc) in H1.
+  apply H2 in H1. hnf; rewrite H1.
+  unfold beyond_block. rewrite resource_at_make_rmap.
+  unfold beyond_block'.
+  rewrite if_false by (  destruct loc; destruct H; subst; simpl; unfold block; omega).
+  unfold inflate_initial_mem. rewrite resource_at_make_rmap.
+  unfold inflate_initial_mem'. rewrite H4.
+ unfold Genv.perm_globvar. rewrite VOL. rewrite preds_fmap_NoneP.
+  destruct (gvar_readonly v);  repeat f_equal; auto.
+  apply read_sh_readonly.
+  rewrite H0.
+  destruct loc; destruct H; subst b0.
+  apply nth_getN; simpl; omega.
+  rewrite H0.
+  destruct loc; destruct H; subst b0.
+  apply nth_getN; simpl; omega.
+
+ repeat split; auto; clear H.
+  simpl in AL. apply Zmod_divide.  intro Hx; inv Hx. apply Zeq_bool_eq; auto.
+  intro loc; specialize (H2 loc).
+  simpl in H2. simpl size_chunk. hnf; if_tac; auto.
+  exists NU.
+  destruct H2.
+  apply join_comm in H1.
+  apply (resource_at_join _ _ _ loc) in H1.
+  apply H2 in H1. hnf; rewrite H1.
+  unfold beyond_block. rewrite resource_at_make_rmap.
+  unfold beyond_block'.
+  rewrite if_false by (  destruct loc; destruct H; subst; simpl; unfold block; omega).
+  unfold inflate_initial_mem. rewrite resource_at_make_rmap.
+  unfold inflate_initial_mem'. rewrite H4.
+ unfold Genv.perm_globvar. rewrite VOL. rewrite preds_fmap_NoneP.
+  destruct (gvar_readonly v);  repeat f_equal; auto.
+  apply read_sh_readonly.
+  rewrite H0.
+  destruct loc; destruct H; subst b0.
+  apply nth_getN; simpl; omega.
+  rewrite H0.
+  destruct loc; destruct H; subst b0.
+  apply nth_getN; simpl; omega.
+
+  intro loc. hnf. specialize (H2 loc); simpl in H2.
+ if_tac; auto.
+    exists NU.
+  destruct H2.
+  apply join_comm in H1.
+  apply (resource_at_join _ _ _ loc) in H1.
+  apply H2 in H1. hnf; rewrite H1.
+  unfold beyond_block. rewrite resource_at_make_rmap.
+  unfold beyond_block'.
+  rewrite if_false by (  destruct loc; destruct H3; subst; simpl; unfold block; omega).
+  unfold inflate_initial_mem. rewrite resource_at_make_rmap.
+  unfold inflate_initial_mem'. rewrite H4.
+ unfold Genv.perm_globvar. rewrite VOL. rewrite preds_fmap_NoneP.
+  destruct loc; destruct H3; subst b0.
+  specialize (H (z1-z)).  spec H; [omega |].
+  if_tac in H; [ | discriminate].
+  replace (z+(z1-z)) with z1 in * by omega.
+  rewrite H0.
+  inv H.
+  assert (contents_at m3 (b,z1) = Byte Byte.zero). 
+    unfold contents_at.
+    simpl. forget (ZMap.get z1 (ZMap.get b (mem_contents m3))) as byt.
+    clear - H7.
+    unfold decode_val in H7. 
+    revert H7; case_eq (proj_bytes (byt::nil)); intros; try discriminate.
+    simpl in  H. destruct byt; inv H.
+    unfold decode_int in H7.
+    replace (rev_if_be (i::nil)) with (i::nil) in H7 by (unfold rev_if_be; destruct big_endian; auto).
+    simpl int_of_bytes in H7.
+    replace (Byte.unsigned i + 0) with (Byte.unsigned i) in H7 by omega.
+    f_equal.
+    admit. (* looks true *)
+  destruct (gvar_readonly v);  repeat f_equal; auto.
+  apply read_sh_readonly.
+  match type of H with Some (decode_val ?ch ?A) = Some ?B => 
+       assert (decode_val ch A=B) by (inv H; auto); clear H; 
+        destruct (Genv.find_symbol ge i); try exists A
+  end.
+  repeat split; auto.
+  simpl in AL. apply Zmod_divide.  intro Hx; inv Hx. apply Zeq_bool_eq; auto.
+  intro loc; specialize (H2 loc). hnf. simpl Genv.init_data_size in H2.
+   simpl size_chunk.
+ if_tac.
+  exists NU. hnf. 
+  destruct H2.
+  apply join_comm in H1.
+  apply (resource_at_join _ _ _ loc) in H1.
+  apply H2 in H1. hnf; rewrite H1.
+  unfold beyond_block. rewrite resource_at_make_rmap.
+  unfold beyond_block'.
+  rewrite if_false by (  destruct loc; destruct H; subst; simpl; unfold block; omega).
+  unfold inflate_initial_mem. rewrite resource_at_make_rmap.
+  unfold inflate_initial_mem'. rewrite H5.
+ unfold Genv.perm_globvar. rewrite VOL. rewrite preds_fmap_NoneP.
+  destruct (gvar_readonly v);  repeat f_equal; auto.
+  apply read_sh_readonly.
+  rewrite H0.
+  destruct loc; destruct H.  subst b1.
+  apply nth_getN; simpl; omega.
+  rewrite H0.
+  destruct loc; destruct H; subst b1.
+  apply nth_getN; simpl; omega.
+  apply H2.
+  intro loc.
+  specialize (H2 loc). simpl in H2.
+  hnf. simpl Genv.init_data_size. rewrite Zmax_left by omega.
+  if_tac. exists NU.
+  destruct H2.
+  apply join_comm in H1.
+  apply (resource_at_join _ _ _ loc) in H1.
+  apply H2 in H1. hnf; rewrite H1.
+  unfold beyond_block. rewrite resource_at_make_rmap.
+  unfold beyond_block'.
+  rewrite if_false by (  destruct loc; destruct H; subst; simpl; unfold block; omega).
+  unfold inflate_initial_mem. rewrite resource_at_make_rmap.
+  unfold inflate_initial_mem'. rewrite H5.
+ unfold Genv.perm_globvar. rewrite VOL. rewrite preds_fmap_NoneP.
+  assert (contents_at m4 loc = Byte Byte.zero).
+    rewrite H0.
+    destruct loc; destruct H; subst b0.
+    rewrite (nth_getN m3 b z z0 4); auto.
+    unfold size_chunk_nat in H4.
+    forget (ZMap.get b (mem_contents m3)) as byt.
+    clear - H4 H6.
+    simpl size_chunk in *. simpl nat_of_Z in *.
+    unfold nat_of_P in *. simpl Pmult_nat in *.
+    assert (0 <= z0-z < 4) by omega.
+    clear - H H4.
+    admit.
+    omega.
+  destruct (gvar_readonly v);  repeat f_equal; auto.
+  apply read_sh_readonly.
+  apply H2.
+Qed.
+
+
+Lemma init_data_list_lem:
+  forall ge m0 (v: globvar type) m1 b m2 m3 m4  phi0,
+     alloc m0 0 (Genv.init_data_list_size (gvar_init v)) = (m1,b) ->
+     Genv.store_zeros m1 b 0 (Genv.init_data_list_size (gvar_init v)) = Some m2 ->
+     Genv.store_init_data_list ge m2 b 0 (gvar_init v) = Some m3 ->
+     drop_perm m3 b 0 (Genv.init_data_list_size (gvar_init v)) 
+               (Genv.perm_globvar v) = Some m4 ->
+     gvar_volatile v = false ->
+   initializers_aligned 0 (gvar_init v) = true ->
+     init_data_list2pred ge (gvar_init v) (readonly2share (gvar_readonly v)) b 0 
+            (beyond_block b (inflate_initial_mem m4 phi0)).
+Proof.
+intros. rename H3 into VOL. rename H4 into AL.
+set (phi := beyond_block b (inflate_initial_mem m4 phi0)).
+assert (forall loc, fst loc <> b -> identity (phi @ loc)).
+  unfold phi; intros.
+  unfold beyond_block. rewrite resource_at_make_rmap.
+  unfold beyond_block'.
+  if_tac. apply core_identity.
+  unfold inflate_initial_mem.  rewrite resource_at_make_rmap.
+  unfold inflate_initial_mem'.
+  unfold access_at.
+  rewrite nextblock_noaccess. apply NO_identity. 
+  rewrite (nextblock_drop _ _ _ _ _ _ H2).
+  rewrite (Genv.store_init_data_list_nextblock _ _ _ _ _ H1).
+  rewrite (Genv.store_zeros_nextblock _ _ _ _ H0).
+  assert (nextblock m1 = Zsucc b /\ b = nextblock m0).
+   clear - H. Transparent alloc. inv H.  simpl. auto. Opaque alloc.
+ destruct H5; unfold block in *; omega.
+ assert (forall loc, if adr_range_dec (b,0)  (Genv.init_data_list_size (gvar_init v)) loc
+                             then access_at m4 loc = Some (Genv.perm_globvar v)
+                             else identity (phi @ loc)).
+  intro. if_tac.
+     destruct loc; destruct H4; subst b0.
+     unfold access_at. simpl. forget (Genv.perm_globvar v) as p.
+      forget (Genv.init_data_list_size (gvar_init v)) as n.
+     clear - H2 H5. unfold drop_perm in H2.
+      destruct (range_perm_dec m3 b 0 n Cur Freeable); inv H2.
+      simpl.  rewrite ZMap.gss.
+       destruct (zle 0 z); try omegaContradiction. destruct (zlt z n); try omegaContradiction.
+       simpl; auto.
+    destruct loc.
+  destruct (eq_dec b b0). subst b0.
+  unfold phi. unfold beyond_block. rewrite resource_at_make_rmap.
+  unfold beyond_block'. simpl. rewrite if_false by (unfold block; omega).
+  unfold inflate_initial_mem.  rewrite resource_at_make_rmap.
+  unfold inflate_initial_mem'.
+  replace (access_at m4 (b,z)) with (@None permission).
+  apply NO_identity.
+  symmetry.  transitivity (access_at m3 (b,z)).
+  clear - H4 H2. unfold access_at; unfold drop_perm in H2.
+   destruct (range_perm_dec m3 b 0 (Genv.init_data_list_size (gvar_init v)) Cur
+         Freeable); inv H2. simpl. rewrite ZMap.gss.
+  unfold adr_range in H4. destruct (zle 0 z); auto.
+   destruct (zlt z (Genv.init_data_list_size (gvar_init v)) ); auto.
+  contradiction H4. split; auto.
+  transitivity (access_at m2 (b,z)).
+  apply store_init_data_list_outside' in H1.
+  destruct H1 as [? [? ?]]; congruence.
+  transitivity (access_at m1 (b,z)).
+  clear - H0. admit.
+  clear - H H4. Transparent alloc. inv H. Opaque alloc. unfold access_at; simpl.
+  rewrite ZMap.gss. destruct (zle 0 z); auto.
+   destruct (zlt z (Genv.init_data_list_size (gvar_init v)) ); auto.
+  contradiction H4. split; auto.
+   apply H3. auto.
+  clear H3.
+  assert (contents_at m4 = contents_at m3).
+  clear - H2; unfold contents_at, drop_perm in *.
+   destruct (range_perm_dec m3 b 0 (Genv.init_data_list_size (gvar_init v)) Cur
+         Freeable); inv H2. simpl. auto.
+   clear H2. 
+   forget (gvar_init v) as dl.
+   remember dl as D.
+   rewrite HeqD in AL,H4|-*.
+   assert (nil++dl=D) by (subst; auto).
+   remember (@nil init_data) as dl'.
+   remember (core phi) as w'.
+   remember phi as w.
+   assert (join w' w phi). subst. apply core_unit.
+   remember 0 as z. rewrite Heqz in H,H0,H1.
+   replace z with (Genv.init_data_list_size dl') in AL,H4|-* by (subst; auto).
+   clear z Heqz.
+   assert (forall loc, if adr_range_dec (b,Genv.init_data_list_size dl') (Genv.init_data_list_size dl) loc 
+                               then identity (w' @ loc)  else identity (w @ loc)).
+  intro. subst. if_tac. rewrite <- core_resource_at. apply core_identity.
+  specialize (H4 loc). rewrite if_false in H4 by auto; auto.
+   clear Heqw' Heqw Heqdl' HeqD.
+   revert dl' w' w AL H2 H4 H5 H6; induction dl; simpl; intros.
+   apply all_resource_at_identity; intro loc.
+   specialize (H6 loc); if_tac in H6; auto. destruct loc; destruct H7.
+  omegaContradiction.
+  destruct (split_range w (b,Genv.init_data_list_size dl') (Genv.init_data_size a)) as [w1 [w2 [? ?]]].
+  intros. apply (resource_at_join _ _ _ loc) in H5.
+  specialize (H6 loc). rewrite if_true in H6. apply H6 in H5.
+  rewrite H5.
+   admit.  (* straightforward *)
+  destruct loc. destruct H7; split; auto.
+  assert (Genv.init_data_list_size dl >= 0) by admit.
+  omega.
+  exists w1; exists w2; split3; auto. 
+  clear IHdl. 
+  destruct (join_assoc H7 (join_comm H5)) as [wf [? ?]].
+  assert (forall loc, if adr_range_dec (b,Genv.init_data_list_size dl') (Genv.init_data_size a) loc
+                                 then identity (wf @ loc) /\ 
+                                         access_at m4 loc = Some (Genv.perm_globvar v)
+                                 else identity (w1 @ loc)).
+     intro. specialize (H8 loc); specialize (H6 loc); specialize (H4 loc).
+       apply (resource_at_join _ _ _ loc) in H9;
+       apply (resource_at_join _ _ _ loc) in H10.
+ if_tac.  rewrite if_true in H6,H4. apply H8 in H9. rewrite <- H9; auto.
+  admit. (* easy *)
+  admit. (* easy *)
+ auto.       
+  pose proof (load_store_init_data_lem1 H0 H1 _ _ _ H2).
+  unfold phi in *; clear phi.
+  eapply init_data_lem; try eassumption.
+  clear - AL. apply andb_true_iff in AL. destruct AL; auto.
+
+  destruct (join_assoc (join_comm H7) (join_comm H5)) as [wg [? ?]].
+  specialize (IHdl  (dl' ++ (a::nil))  wg w2).
+  replace (Genv.init_data_list_size (dl' ++ a :: nil)) with
+             (Genv.init_data_list_size dl' + Genv.init_data_size a) in IHdl.
+  apply IHdl; auto.
+  apply andb_true_iff in AL; destruct AL; auto.
+  rewrite app_ass; auto.
+  intro loc; specialize (H6 loc); specialize (H8 loc); specialize (H4 loc).
+  if_tac. rewrite if_true in H4; auto.
+  destruct loc; destruct H11; auto.
+  split; auto. 
+  assert (Genv.init_data_size a >= 0) by admit.
+  omega.
+  if_tac in H8; auto.
+  rewrite if_false in H6.
+  apply join_comm in H5.
+  apply (resource_at_join _ _ _ loc) in H7.
+  apply H8 in H7. rewrite H7; auto.
+  destruct loc.
+  intros [? ?]. subst b0.
+  forget (Genv.init_data_list_size dl') as u.
+ destruct (zlt z (u + Genv.init_data_size a)).
+ apply H12.  split; auto. omega.
+ apply H11.  split; auto. omega.
+  intro loc. specialize (H4 loc); specialize (H6 loc); specialize (H8 loc).
+  apply (resource_at_join _ _ _ loc) in H7.
+  apply (resource_at_join _ _ _ loc) in H9.
+  apply (resource_at_join _ _ _ loc) in H10.
+  apply (resource_at_join _ _ _ loc) in H5.
+ destruct loc.
+  if_tac in H8.
+  rewrite if_false; auto.
+ clear - H11; destruct H11; intros [? ?]. omega.
+  if_tac in H4.
+  rewrite if_true.
+  apply H8 in H9. rewrite <- H9 in *. auto.
+  destruct H12; subst b0. split; auto. 
+  forget (Genv.init_data_list_size dl') as u.
+  assert (~ (u <= z < u + Genv.init_data_size a)) by (contradict H11; destruct H11; split; auto; omega).
+  omega.
+ rewrite if_false. apply H8 in H7. rewrite H7; auto.
+ contradict H12. destruct H12; split; auto.
+   assert (Genv.init_data_size a >= 0) by admit.
+ omega.
+ clear.
+  induction dl'; simpl; intros; try omega.
+Qed.
+
+Definition all_initializers_aligned (prog: AST.program fundef type) := 
+  forallb (fun idv => initializers_aligned 0 (gvar_init (snd idv))) (prog_vars prog) = true.
+
+Lemma forallb_rev: forall {A} f (vl: list A), forallb f (rev vl) = forallb f vl.
+Proof. induction vl; simpl; auto.
+  rewrite forallb_app. rewrite IHvl. simpl. rewrite andb_comm.
+  rewrite <- andb_assoc. f_equal; auto.
+Qed.
+
+Lemma global_initializers:
+  forall prog G m n,
+     list_norepet (prog_defs_names prog) ->
+     all_initializers_aligned prog ->
+    match_fdecs (prog_funct prog) G ->
+    Genv.init_mem prog = Some m ->
+     app_pred (globvars2pred (Genv.globalenv prog) (prog_vars prog))
+  (inflate_initial_mem m (initial_core (Genv.globalenv prog) G n)).
+Proof.
+ intros until n. intros ? AL SAME_IDS ?.
+ unfold all_initializers_aligned in AL.
+ assert (IOK: initial_rmap_ok m (initial_core (Genv.globalenv prog) G n))
+      by (apply initial_core_ok; auto).
+  unfold Genv.init_mem in H0.
+  unfold Genv.globalenv in *.
+  destruct prog as [fl main vl].
+  simpl in *.
+  remember (Genv.add_globals (Genv.empty_genv fundef type) fl) as gev.
+  rewrite <- (rev_involutive fl) in *.
+  rewrite alloc_globals_rev_eq in H0.
+  forget (rev fl) as vl'. clear fl; rename vl' into vl.
+  unfold prog_vars in AL|-*. simpl in AL|-*.
+  rewrite <- rev_prog_vars' in AL|-*.
+  rewrite globvars2pred_rev.
+  rewrite forallb_rev in AL.
+  assert (exists ul, gev = Genv.add_globals (Genv.empty_genv fundef type) (rev vl ++ ul) /\
+                              map fst (prog_funct' (rev vl ++ ul )) = map fst G /\
+                              list_norepet (map (@fst _ _) (rev vl ++ ul))).
+  exists nil; rewrite <- app_nil_end; auto.
+  split; auto. split; auto.
+     clear - SAME_IDS.
+     unfold match_fdecs,prog_funct in SAME_IDS.
+     simpl in SAME_IDS.
+     forget (prog_funct' (rev vl)) as vl'.
+     revert vl' SAME_IDS; induction G; destruct vl'; simpl; intros; auto.
+     inv SAME_IDS. inv SAME_IDS. inv SAME_IDS; f_equal; auto.
+  clear SAME_IDS. 
+  clear IOK; assert (IOK: True) by auto.
+  clear H Heqgev.
+  revert m H0 H1 IOK; induction vl; simpl; intros.
+ apply resource_at_empty2.
+ intro l.
+ unfold inflate_initial_mem.
+ rewrite resource_at_make_rmap.
+ unfold inflate_initial_mem'.
+  inv H0.
+ unfold access_at, empty. simpl. rewrite ZMap.gi. apply NO_identity.
+ invSome.
+ destruct a; destruct g.
+(* Gfun case *) 
+ specialize (IHvl AL _ H0).
+ spec IHvl.
+ destruct H1 as [ul [? [? ?]]].
+ exists ((i,Gfun f)::ul).
+ subst gev.
+ split3.
+ f_equal. rewrite app_ass. simpl; auto.
+ clear - H1. rewrite app_ass in H1. apply H1.
+ rewrite app_ass in H2. apply H2.
+ spec IHvl. auto.
+ admit. (* quite possibly true, because the only difference
+    between (inflate_initial_mem m0 ...) and (inflate_initial_mem m ...)
+    is a PURE at a location where globvars2pred will yield emp *)
+(* Gvar case *)
+  spec IHvl.
+ clear - AL. simpl in AL. apply andb_true_iff in AL. destruct AL; auto.
+ specialize (IHvl _ H0).
+ unfold globvars2pred. simpl map.
+ unfold Genv.alloc_global in H3.
+ revert H3; case_eq (alloc m0 0 (Genv.init_data_list_size (gvar_init v))); intros.
+ invSome. invSome.
+ destruct H1 as [ul [? [? ?]]].
+ spec IHvl.
+  exists ((i, Gvar v)::ul).
+ rewrite app_ass in H1,H2,H4; split3; auto.
+ unfold globvar2pred at 1. simpl @fst; simpl @snd.
+ spec IHvl. auto.
+ assert (Genv.find_symbol gev i = Some b).
+   apply alloc_result in H. subst.
+ rewrite <- alloc_globals_rev_eq in H0. 
+ apply Genv.alloc_globals_nextblock in H0.
+ rewrite H0.
+ rewrite app_ass in *. simpl app in *.
+ simpl nextblock.
+ apply add_variables_nextblock; auto. 
+ rewrite H7.
+ case_eq (gvar_volatile v); intros.
+ admit.  (* very likely true *)
+ simpl fold_right.
+ set (phi:= inflate_initial_mem m (initial_core gev G n)) in *.
+ exists (beyond_block b phi), (upto_block b phi).
+ split3.
+ clear.  admit.  (* easy; make a lemma *)
+ eapply init_data_list_lem; try eassumption.
+ clear - AL. simpl in AL. apply andb_true_iff in AL; destruct AL; auto.
+ change (globvars2pred gev (prog_vars' vl) (upto_block b phi)).
+ replace (upto_block b phi) with (inflate_initial_mem m0 (initial_core gev G n)); auto.
+ unfold phi in *; clear phi.
+ clear - H H3 H5 H6.
+ apply rmap_ext.
+ clear.  admit.  (* easy; make a lemma for upto_block *)
+ intro loc.
+ unfold upto_block. rewrite resource_at_make_rmap. unfold upto_block'.
+ unfold inflate_initial_mem.
+ repeat rewrite resource_at_make_rmap.
+ if_tac. 
+ unfold inflate_initial_mem'.
+ replace (access_at m0 loc) with (access_at m loc); auto.
+ replace (contents_at m0 loc) with (contents_at m loc); auto.
+ admit.  (* easy *)
+ admit.  (* easy *)
+ unfold inflate_initial_mem'.
+ replace (access_at m0 loc) with (@None permission); auto.
+ symmetry.
+ admit.  (* easy *)
+Qed.
+
+Lemma disj_no_fun:  (* do we still need this? *)
+  forall (fs: list (AST.ident * globdef fundef type)) ids, 
+       list_disjoint (map (@fst _ _) fs) ids ->
+       forall i, In i ids ->
+      (Genv.genv_symb (Genv.add_globals (Genv.empty_genv _ _) fs)) ! i = None.
+Proof.
+intros. spec H i i.
+assert (~In i (map (@fst _ _) fs)). intro. contradiction H; auto.
+clear - H1; rename H1 into H0. unfold Genv.add_globals.
+rewrite fold_right_rev_left. rewrite <- (rev_involutive fs). rewrite In_rev in H0.
+rewrite <- map_rev in H0. remember (rev fs) as fs'; rewrite rev_involutive. clear - H0.
+revert H0; induction fs'; simpl; intros.
+rewrite Maps.PTree.gempty; auto. destruct a; simpl in *.
+rewrite Maps.PTree.gso; [ | intro; subst; intuition]. 
+apply IHfs'. contradict H0; auto.
+Qed.
